example2b.bpl
@@ -1,0 +1,906 @@
+type Ref;
+type Transaction;
+type Stack = [int] Ref;
+const unique zero: Ref;
+
+// TypeEnum constants
+// These are configured on the 'verify' procedur. TODO: Configure all
+var Payment: Ref;
+var KeyRegistration: Ref;
+var AssetConfig: Ref;
+var AssetTransfer: Ref;
+var AssetFreeze: Ref;
+var ApplicationCall: Ref;
+
+
+// OnComplete constants
+const Noop : int;
+const OptIn: int;
+const CloseOut: int;
+const ClearState: int;
+const UpdateApplication: int;
+const DeleteApplication: int;
+
+// tx state
+var Alloc: [Ref] bool;
+var GlobalsAlloc: [Ref] bool;
+var Globals: [Ref] Ref;
+var GlobalsExAlloc: [Ref][Ref] bool;
+var GlobalsEx: [Ref][Ref] Ref;
+var LocalsAlloc: [Ref][Ref] bool;
+var Locals: [Ref][Ref] Ref;
+var LocalsExAlloc: [Ref][Ref][Ref] bool;
+var LocalsEx: [Ref][Ref][Ref] Ref;
+var ScratchSpace: [int] Ref;
+var ScratchSpaceAlloc: [int] bool;
+var StackPointer: int;
+var Stack: [int] Ref;
+var IsInt: [Ref] bool;
+var RefToInt: [Ref] int;
+var AssetBalance: [Ref] [int] int; // account, assetId
+var AssetFrozen: [Ref] [int] int; // account, assetId
+var OptedInApp: [Ref] [int] int; // account, appId
+var OptedInAsset: [Ref] [int] int; // account, assetId
+
+var GroupSize: int;
+var Round: int;
+
+// Modeling txns
+var GroupIndex: [Transaction] int;
+var CurrentTxn: Transaction;
+var GroupTransaction: [int] Transaction;
+var Sender : [Transaction] Ref;
+var NumAppArgs : [Transaction] Ref;
+var ApplicationArgs : [Transaction] [int] Ref;
+var OnCompletion : [Transaction] Ref;
+var Accounts : [Transaction] [int] Ref;
+var ApplicationID : [Transaction] Ref;
+var TypeEnum: [Transaction] Ref;
+var AssetReceiver: [Transaction] Ref;
+var XferAsset: [Transaction] Ref;
+var AssetAmount: [Transaction] Ref;
+
+const unique Creator : Ref;
+const unique NotCreator : Ref;
+
+var _: Ref;
+
+// declare srings
+var creator: Ref;
+var regBegin: Ref;
+var regEnd: Ref;
+var voteBegin: Ref;
+var voteEnd: Ref;
+var register: Ref;
+var vote: Ref;
+var voted: Ref;
+var candidatea: Ref;
+var candidateb: Ref;
+
+procedure FreshRefGenerator() returns (newRef: Ref);
+  modifies Alloc;
+  modifies IsInt;
+  //ensures old(Alloc[newRef] == false);
+  //ensures Alloc[newRef] == true;
+  //ensures newRef != zero;
+  //ensures IsInt[newRef] == false;
+  //ensures (forall ref: Ref :: ref != newRef ==> IsInt[ref] == old(IsInt[ref]));
+  //ensures (forall ref: Ref :: ref != newRef ==> Alloc[ref] == old(Alloc[ref]));
+implementation FreshRefGenerator() returns (newRef: Ref) {
+    havoc newRef;
+    assume Alloc[newRef] == false;
+    Alloc[newRef] := true;
+    IsInt[newRef] := false;
+    assume newRef != zero;
+  }
+
+procedure Push(value: Ref, stack: Stack, stackPointer: int) returns (newStack: Stack, newStackPointer: int);
+implementation Push(value: Ref, stack: Stack, stackPointer: int) returns (newStack: Stack, newStackPointer: int){
+  newStackPointer := stackPointer + 1;
+  newStack := stack[stackPointer] := value;
+  }
+
+procedure Pop(stack: [int] Ref, stackPointer: int) returns (top: Ref);
+implementation Pop(stack: [int] Ref, stackPointer: int) returns (top: Ref){
+  top := stack[stackPointer];
+  stackPointer := stackPointer - 1;
+  }
+
+//procedure Store(i: int, stack: [int] Ref, stackPointer: int);
+//  requires 0 <= i ;
+//  requires i < 64;
+//  requires StackPointer >= 0;
+//implementation Store(i: int) {
+//  var value: Ref;
+//  call value := Pop();
+//  ScratchSpaceAlloc[i] := true;
+//  ScratchSpace[i] := value;
+//  }
+//
+//procedure Load(i: int);
+//  requires 0 <= i ;
+//  requires i < 64;
+//  requires ScratchSpaceAlloc[i] == true;
+//  modifies Stack;
+//  modifies StackPointer;
+//  //ensures Stack[StackPointer] == ScratchSpace[i];
+//  //ensures StackPointer == old(StackPointer)+1;
+//  //ensures (forall j: int:: -1 <= j && j < StackPointer ==> Stack[j] == old(Stack[j]));
+//  //ensures (forall j: int:: 0 < j && j < 64 && i != j ==> ScratchSpaceAlloc[j] == old(ScratchSpaceAlloc[j]));
+//implementation Load(i: int) {
+//  call Push(ScratchSpace[i]);
+//  }
+//
+//// Returns any Ref
+//procedure AppGlobalGetEx();
+//  requires StackPointer > 0;
+//implementation AppGlobalGetEx() {
+//  //var value: Ref;
+//  //var _: Ref;
+//  //havoc value;
+//  //call _ := Pop();
+//  //call _ := Pop();
+//  //call Push(value);
+//  call Int(1);
+//  }
+//
+//// Returns any Ref
+//procedure AppLocalGetEx();
+//  requires StackPointer > 0;
+//implementation AppLocalGetEx() {
+//  //var value: Ref;
+//  //var _: Ref;
+//  //havoc value;
+//  //call _ := Pop();
+//  //call _ := Pop();
+//  //call _ := Pop();
+//  //call Push(value);
+//  call Int(0);
+//  }
+
+procedure AppGlobalGet(stack: [int] Ref, stackPointer: int);
+implementation AppGlobalGet(stack: [int] Ref, stackPointer: int) {
+  var value: Ref;
+  var key: Ref;
+  value := zero;
+  call key := Pop(stack, stackPointer);
+  if (GlobalsAlloc[key] == true) {
+    value := Globals[key];
+    }
+  call Push(value, stack, stackPointer);
+  }
+
+procedure AppGlobalPut(stack: [int] Ref, stackPointer: int);
+  requires StackPointer > 0;
+  modifies Globals;
+  modifies GlobalsAlloc;
+  modifies Stack;
+  modifies StackPointer;
+  //ensures GlobalsAlloc[old(Stack[old(StackPointer)-1])] == true;
+  //ensures Globals[old(Stack[old(StackPointer)-1])] == old(Stack[old(StackPointer)]);
+  //ensures StackPointer == old(StackPointer) - 2;
+  //ensures (forall i: int:: -1 <= i && i <= StackPointer ==> Stack[i] == old(Stack[i]));
+  //ensures (forall ref: Ref :: ref != old(Stack[old(StackPointer)-1]) ==> Globals[ref] == old(Globals[ref]));
+  //ensures (forall ref: Ref :: ref != old(Stack[old(StackPointer)-1]) ==> GlobalsAlloc[ref] == old(GlobalsAlloc[ref]));
+implementation AppGlobalPut(stack: [int] Ref, stackPointer: int) {
+  var value: Ref;
+  var key: Ref;
+  call value := Pop(stack, stackPointer);
+  call key := Pop(stack, stackPointer);
+  GlobalsAlloc[key] := true;
+  Globals[key] := value;
+  }
+
+//procedure Dup();
+//  requires StackPointer >= 0;
+//  modifies Stack;
+//  modifies StackPointer;
+//  //ensures Stack[old(StackPointer)] == old(Stack[old(StackPointer)]);
+//  //ensures Stack[StackPointer] == old(Stack[old(StackPointer)]);
+//  //ensures StackPointer == old(StackPointer) + 1;
+//  //ensures (forall i: int:: -1 <= i && i < StackPointer ==> Stack[i] == old(Stack[i]));
+//implementation Dup() {
+//  call Push(Stack[StackPointer]);
+//  }
+
+procedure Int(n: int, stack: [int] Ref, stackPointer: int);
+  requires n >= 0;
+implementation Int(n: int, stack: [int] Ref, stackPointer: int) {
+  var newRef: Ref;
+  call newRef := FreshRefGenerator();
+  IsInt[newRef] := true;
+  RefToInt[newRef] := n;
+  call Push(newRef, stack, stackPointer);
+  }
+
+//procedure Sum();
+//  requires StackPointer > 0;
+//  requires IsInt[Stack[StackPointer]];
+//  requires IsInt[Stack[StackPointer-1]];
+//  requires RefToInt[Stack[StackPointer]] >= 0;
+//  requires RefToInt[Stack[StackPointer-1]] >= 0;
+//  modifies IsInt;
+//  modifies Alloc;
+//  modifies StackPointer;
+//  modifies Stack;
+//  modifies RefToInt;
+//  //ensures RefToInt[Stack[StackPointer]] == old(RefToInt[old(Stack[old(StackPointer)])]) + old(RefToInt[old(Stack[old(StackPointer)-1])]);
+//  //ensures StackPointer == old(StackPointer) - 1;
+//  //ensures (forall i: int:: -1 <= i && i < StackPointer ==> Stack[i] == old(Stack[i]));
+//  //ensures (forall ref: Ref :: ref != old(Stack[old(StackPointer)]) && ref != old(Stack[old(StackPointer)-1]) && ref != Stack[StackPointer] ==> RefToInt[ref] == old(RefToInt[ref]));
+//  //ensures (forall ref: Ref :: ref != old(Stack[old(StackPointer)]) && ref != old(Stack[old(StackPointer)-1]) && ref != Stack[StackPointer] ==> IsInt[ref] == old(IsInt[ref]));
+//implementation Sum() {
+//  var aRef: Ref;
+//  var bRef: Ref;
+//  call aRef := Pop();
+//  call bRef := Pop();
+//  call Int(RefToInt[aRef] + RefToInt[bRef]);
+//  }
+
+procedure Byte(ref : Ref, stack: [int] Ref, stackPointer: int);
+implementation Byte(ref : Ref, stack: [int] Ref, stackPointer: int) {
+  call Push(ref, stack, stackPointer);
+  }
+
+//procedure Btoi();
+//implementation Btoi() {
+//  var top : Ref;
+//  var n: int;
+//  call top := Pop();
+//  call Int(RefToInt[top]);
+//}
+//
+procedure Return(stack: [int] Ref, stackPointer: int);
+implementation Return(stack: [int] Ref, stackPointer: int){
+  assert !IsInt[stack[stackPointer]] || RefToInt[stack[stackPointer]] > 0;
+}
+
+procedure GTxn(index:int, field: [Transaction] Ref, stack: [int] Ref, stackPointer: int);
+implementation GTxn(index: int, field: [Transaction] Ref, stack: [int] Ref, stackPointer: int) {
+  call Push(field[GroupTransaction[index]], stack, stackPointer);
+  }
+
+procedure Txn(field: [Transaction] Ref, stack: [int] Ref, stackPointer: int);
+implementation Txn(field: [Transaction] Ref, stack: [int] Ref, stackPointer: int) {
+  call GTxn(GroupIndex[CurrentTxn], field, stack, stackPointer);
+  }
+
+//procedure Txna(arrayField: [Transaction][int] Ref, index: int);
+//  modifies Stack;
+//  modifies StackPointer;
+//  //ensures StackPointer == old(StackPointer) + 1;
+//  //ensures Stack[StackPointer] == arrayField[CurrentTxn][index];
+//  //ensures (forall i: int:: -1 <= i && i < StackPointer ==> Stack[i] == old(Stack[i]));
+//implementation Txna(arrayField: [Transaction][int] Ref, index: int) {
+//  call Push(arrayField[CurrentTxn][index]);
+//  }
+
+procedure Equal(stack: [int] Ref, stackPointer: int);
+implementation Equal(stack: [int] Ref, stackPointer: int) {
+    var aRef: Ref;
+    var bRef: Ref;
+    call bRef := Pop(stack, stackPointer);
+    call aRef := Pop(stack, stackPointer);
+    if (aRef == bRef || (IsInt[aRef] && RefToInt[aRef] == RefToInt[bRef])) {
+      call Int(1, stack, stackPointer);
+      return;
+    }
+    call Int(0, stack, stackPointer);
+    return;
+  }
+
+procedure And(stack: [int] Ref, stackPointer: int);
+implementation And(stack: [int] Ref, stackPointer: int) {
+    var aRef: Ref;
+    var bRef: Ref;
+    call bRef := Pop(stack, stackPointer);
+    call aRef := Pop(stack, stackPointer);
+    if (IsInt[aRef] && IsInt[bRef] && RefToInt[aRef] > 0 && RefToInt[bRef] > 0) {
+      call Int(1, stack, stackPointer);
+      return;
+    }
+    call Int(0, stack, stackPointer);
+    return;
+  }
+
+//procedure Or();
+//  requires StackPointer > 0;
+//  requires IsInt[Stack[StackPointer]];
+//  requires IsInt[Stack[StackPointer-1]];
+//implementation Or() {
+//    var aRef: Ref;
+//    var bRef: Ref;
+//    call bRef := Pop();
+//    call aRef := Pop();
+//    if (IsInt[aRef] && IsInt[bRef] && (RefToInt[aRef] > 0 || RefToInt[bRef] > 0)) {
+//      call Int(1);
+//      return;
+//    }
+//    call Int(0);
+//    return;
+//  }
+//
+//procedure GreatOrEqual();
+//  requires StackPointer > 0;
+//  requires IsInt[Stack[StackPointer]];
+//  requires IsInt[Stack[StackPointer-1]];
+//implementation GreatOrEqual() {
+//    var aRef: Ref;
+//    var bRef: Ref;
+//    call bRef := Pop();
+//    call aRef := Pop();
+//    if (RefToInt[aRef] >= RefToInt[bRef]) {
+//      call Int(1);
+//      return;
+//    }
+//    call Int(0);
+//    return;
+//  }
+//
+//procedure LessOrEqual();
+//  requires StackPointer > 0;
+//  requires IsInt[Stack[StackPointer]];
+//  requires IsInt[Stack[StackPointer-1]];
+//implementation LessOrEqual() {
+//    var aRef: Ref;
+//    var bRef: Ref;
+//    call bRef := Pop();
+//    call aRef := Pop();
+//    if (RefToInt[aRef] <=  RefToInt[bRef]) {
+//      call Int(1);
+//      return;
+//    }
+//    call Int(0);
+//    return;
+//  }
+//
+//procedure AppOptedIn();
+//  requires StackPointer > 0;
+//  requires IsInt[Stack[StackPointer]];
+//  requires IsInt[Stack[StackPointer-1]];
+//implementation AppOptedIn() {
+//    var applicationIDRef: Ref;
+//    var accountsIndexRef: Ref;
+//    var accountRef: Ref;
+//    var applicationID: int;
+//
+//    call applicationIDRef := Pop();
+//    call accountsIndexRef := Pop();
+//
+//    applicationID := RefToInt[applicationIDRef];
+//    accountRef := Accounts[CurrentTxn][RefToInt[accountsIndexRef]];
+//
+//    if (OptedInApp[accountRef][applicationID] > 0) {
+//      call Int(1);
+//      return;
+//    }
+//    call Int(0);
+//    return;
+//  }
+//
+//procedure AssetHoldingGet(field: [Ref][int]int);
+//  requires StackPointer > 0;
+//  requires IsInt[Stack[StackPointer]];
+//  requires IsInt[Stack[StackPointer-1]];
+//implementation AssetHoldingGet(field: [Ref][int]int) {
+//    var assetIdRef: Ref;
+//    var accountsIndexRef: Ref;
+//    var accountRef: Ref;
+//    var assetId: int;
+//
+//    call accountRef := FreshRefGenerator();
+//    call assetIdRef := Pop();
+//    call accountsIndexRef := Pop();
+//
+//    assetId := RefToInt[assetIdRef];
+//    assert RefToInt[accountsIndexRef] == 0;
+//    assert Accounts[CurrentTxn][0] == Sender[CurrentTxn];
+//    assert Accounts[CurrentTxn][RefToInt[accountsIndexRef]] == Sender[CurrentTxn];
+//    assert NotCreator == Sender[CurrentTxn];
+//    accountRef := Accounts[CurrentTxn][RefToInt[accountsIndexRef]];
+//    assert field[accountRef][assetId]>= 1;
+//    call Int(field[accountRef][assetId]);
+//    if (OptedInAsset[accountRef][assetId] > 0) {
+//      call Int(1);
+//      return;
+//    }
+//    call Int(0);
+//    return;
+//  }
+
+
+
+procedure contract();
+implementation contract() {
+  call Int(0, Stack, StackPointer);
+  call Txn(ApplicationID, Stack, StackPointer);
+  call Equal(Stack, StackPointer);
+  if (IsInt[Stack[StackPointer]] && RefToInt[Stack[StackPointer]] == 0) {
+    goto not_creation;
+  }
+  call Byte(creator, Stack, StackPointer);
+  call Txn(Sender, Stack, StackPointer);
+  call AppGlobalPut(Stack, StackPointer);
+  call Txn(NumAppArgs, Stack, StackPointer);
+  call Int(4, Stack, StackPointer);
+  call Equal(Stack, StackPointer);
+  if (IsInt[Stack[StackPointer]] && RefToInt[Stack[StackPointer]] == 0) {
+    goto failed;
+  }
+//  call Byte(regBegin);
+//  call Txna(ApplicationArgs, 0);
+//  call Btoi();
+//  call AppGlobalPut();
+//  call Byte(regEnd);
+//  call Txna(ApplicationArgs, 1);
+//  call Btoi();
+//  call AppGlobalPut();
+//  call Byte(voteBegin);
+//  call Txna(ApplicationArgs, 2);
+//  call Btoi();
+//  call AppGlobalPut();
+//  call Byte(voteEnd);
+//  call Txna(ApplicationArgs, 3);
+//  call Btoi();
+//  call AppGlobalPut();
+//  call Int(1);
+//  call Return();
+//  return;
+  not_creation:
+    return;
+//    call Int(DeleteApplication);
+//    call Txn(OnCompletion);
+//    call Equal();
+//    if (IsInt[Stack[StackPointer]] && RefToInt[Stack[StackPointer]] == 0) {
+//      goto not_deletion;
+//    }
+//    call Byte(creator);
+//    call AppGlobalGet();
+//    call Txn(Sender);
+//    call Equal();
+//    if (IsInt[Stack[StackPointer]] && RefToInt[Stack[StackPointer]] == 0) {
+//      goto failed;
+//    }
+//    call Int(1);
+//    call Return();
+//    return;
+//  not_deletion:
+//    call Int(UpdateApplication);
+//    call Txn(OnCompletion);
+//    call Equal();
+//    if (IsInt[Stack[StackPointer]] && RefToInt[Stack[StackPointer]] == 0) {
+//      goto not_update;
+//    }
+//    call Byte(creator);
+//    call AppGlobalGet();
+//    call Txn(Sender);
+//    call Equal();
+//    if (IsInt[Stack[StackPointer]] && RefToInt[Stack[StackPointer]] == 0) {
+//      goto failed;
+//    }
+//    call Int(1);
+//    call Return();
+//    return;
+//  not_update:
+//    call Int(CloseOut);
+//    call Txn(OnCompletion);
+//    call Equal();
+//    if (IsInt[Stack[StackPointer]] && RefToInt[Stack[StackPointer]] != 0) {
+//      goto close_out;
+//    }
+//    call Txna(ApplicationArgs,0);
+//    call Byte(register);
+//    call Equal();
+//    if (IsInt[Stack[StackPointer]] && RefToInt[Stack[StackPointer]] != 0) {
+//      goto register;
+//    }
+//    call Txna(ApplicationArgs,0);
+//    call Byte(vote);
+//    call Equal();
+//    if (IsInt[Stack[StackPointer]] && RefToInt[Stack[StackPointer]] != 0) {
+//      goto vote;
+//    }
+//    call Int(0);
+//    call Return();
+//    return;
+//  vote:
+//    // global Round
+//    call Int(Round);
+//    call Byte(voteBegin);
+//    call AppGlobalGet();
+//    call GreatOrEqual();
+//    call Int(Round);
+//    assert voteEnd != zero;
+//    assert !IsInt[voteEnd];
+//    call Byte(voteEnd);
+//    call AppGlobalGet();
+//    call LessOrEqual();
+//    call And();
+//    if (IsInt[Stack[StackPointer]] && RefToInt[Stack[StackPointer]] == 0) {
+//      goto failed;
+//    }
+//    call Int(0);
+//    call Txn(ApplicationID);
+//    call AppOptedIn();
+//    if (IsInt[Stack[StackPointer]] && RefToInt[Stack[StackPointer]] == 0) {
+//      goto failed;
+//    }
+//    call Int(0);
+//    call Int(2);
+//    call AssetHoldingGet(AssetBalance);
+//    call _ := Pop();
+//    call Int(1);
+//    call GreatOrEqual();
+//    if (IsInt[Stack[StackPointer]] && RefToInt[Stack[StackPointer]] == 0) {
+//      goto failed;
+//    }
+//    call Int(GroupSize);
+//    call Int(2);
+//    call Equal();
+//    if (IsInt[Stack[StackPointer]] && RefToInt[Stack[StackPointer]] == 0) {
+//      goto failed;
+//    }
+//    call GTxn(1,TypeEnum);
+//    call Int(4);
+//    // TODO: should fail here
+//    call Equal();
+//    if (IsInt[Stack[StackPointer]] && RefToInt[Stack[StackPointer]] == 0) {
+//      goto failed;
+//    }
+//    call Byte(creator);
+//    call AppGlobalGet();
+//    call GTxn(1,AssetReceiver);
+//    call Equal();
+//    if (IsInt[Stack[StackPointer]] && RefToInt[Stack[StackPointer]] == 0) {
+//      goto failed;
+//    }
+//    call GTxn(1,XferAsset);
+//    call Int(2);
+//    call Equal();
+//    if (IsInt[Stack[StackPointer]] && RefToInt[Stack[StackPointer]] == 0) {
+//      goto failed;
+//    }
+//    call GTxn(1,AssetAmount);
+//    call Int(1);
+//    call Equal();
+//    if (IsInt[Stack[StackPointer]] && RefToInt[Stack[StackPointer]] == 0) {
+//      goto failed;
+//    }
+//    call Int(0);
+//    call Txn(ApplicationID);
+//    call Byte(voted);
+//    call AppLocalGetEx();
+//    if (IsInt[Stack[StackPointer]] && RefToInt[Stack[StackPointer]] != 0) {
+//      goto voted;
+//    }
+//    call _ := Pop();
+//    call Txna(ApplicationArgs, 1);
+//    call Byte(candidatea);
+//    call Equal();
+//    call Txna(ApplicationArgs, 1);
+//    call Byte(candidateb);
+//    call Equal();
+//    call Or();
+//    if (IsInt[Stack[StackPointer]] && RefToInt[Stack[StackPointer]] == 0) {
+//      goto failed;
+//    }
+//    call Int(0);
+//    call Txna(ApplicationArgs,1);
+//    call AppGlobalGetEx();
+//    if (IsInt[Stack[StackPointer]] && RefToInt[Stack[StackPointer]] != 0) {
+//      goto increment_existing;
+//    }
+//    call _:= Pop();
+//    call Int(0);
+//  increment_existing:
+//    call Int(1);
+//    call Sum();
+//    call Store(1);
+//    call Txna(ApplicationArgs,1);
+//    call Load(1);
+//    call AppGlobalPut();
+//    call Int(0);
+//    call Byte(voted);
+//    call Txna(ApplicationArgs,1);
+//    call AppGlobalPut();
+//    call Int(1);
+//    call Return();
+//    return;
+//  voted:
+//    call _ := Pop();
+//    call Int(1);
+//    call Return();
+//    return;
+//  register:
+//    call Int(Round);
+//    call Byte(regBegin);
+//    call AppGlobalGet();
+//    call GreatOrEqual();
+//    call Int(Round);
+//    call Byte(regEnd);
+//    call AppGlobalGet();
+//    call LessOrEqual();
+//    call And();
+//    call Int(OptIn);
+//    call Txn(OnCompletion);
+//    call Equal();
+//    call And();
+//    if (IsInt[Stack[StackPointer]] && RefToInt[Stack[StackPointer]] == 0) {
+//      goto failed;
+//    }
+//    call Int(1);
+//    call Return();
+//    return;
+//  close_out:
+//    call Int(1);
+//    call Return();
+//    return;
+  failed:
+    call Int(0,Stack, StackPointer);
+    call Return(Stack, StackPointer);
+    return;
+  }
+
+
+procedure verify();
+  requires GroupSize > 0;
+  requires (forall txn: Transaction:: 0 <= GroupIndex[txn]);
+  requires (forall txn: Transaction:: GroupIndex[txn] < GroupSize);
+  requires (forall txn: Transaction:: GroupTransaction[GroupIndex[txn]] == txn);
+  requires Accounts[CurrentTxn][0] == Sender[CurrentTxn];
+  requires OptIn > 0;
+  requires CloseOut > 0;
+  requires DeleteApplication > 0;
+  requires UpdateApplication > 0;
+  requires StackPointer == -1;
+implementation verify() {
+  // get string refs
+  call creator := FreshRefGenerator();
+  call regBegin := FreshRefGenerator();
+  call regEnd := FreshRefGenerator();
+  call voteBegin := FreshRefGenerator();
+  call voteEnd := FreshRefGenerator();
+  call register := FreshRefGenerator();
+  call vote := FreshRefGenerator();
+  call voted := FreshRefGenerator();
+  call candidatea := FreshRefGenerator();
+  call candidateb := FreshRefGenerator();
+
+  assume IsInt[zero] == true;
+  assume RefToInt[zero] == 0;
+  assume Alloc[zero];
+  assume Alloc[Creator];
+  assume Alloc[NotCreator];
+  assume Alloc[AssetTransfer];
+  assume IsInt[AssetTransfer];
+  assume RefToInt[AssetTransfer] == 4;
+
+  assume Noop == 0;
+  assume OptIn == 1;
+  assume CloseOut == 2;
+  assume ClearState == 3;
+  assume UpdateApplication == 4;
+  assume DeleteApplication == 5;
+
+  call verifyCreation();
+  // call verifyDeleteApplication();
+  // call verifyUpdateApplication();
+  // call verifyCloseOut();
+  // call verifyRegister();
+  call verifyVote();
+  assert false;
+}
+
+procedure verifyCreation();
+implementation verifyCreation() {
+  var numAppArgs : Ref;
+  var onCompletion : Ref;
+  var applicationArgs0 : Ref;
+  var applicationArgs1 : Ref;
+  var applicationArgs2 : Ref;
+  var applicationArgs3 : Ref;
+  var applicationID : Ref;
+
+  call numAppArgs := FreshRefGenerator();
+  call applicationArgs0 := FreshRefGenerator();
+  call applicationArgs1 := FreshRefGenerator();
+  call applicationArgs2 := FreshRefGenerator();
+  call applicationArgs3 := FreshRefGenerator();
+  call applicationID := FreshRefGenerator();
+  call onCompletion := FreshRefGenerator();
+
+  IsInt[applicationID] := true;
+  ApplicationID[CurrentTxn] := applicationID;
+  RefToInt[ApplicationID[CurrentTxn]] := 0;
+
+  Sender[CurrentTxn] := Creator;
+
+  IsInt[numAppArgs] := true;
+  NumAppArgs[CurrentTxn] := numAppArgs;
+  RefToInt[NumAppArgs[CurrentTxn]] := 4;
+
+  IsInt[onCompletion] := true;
+  OnCompletion[CurrentTxn] := onCompletion;
+
+  ApplicationArgs[CurrentTxn][0] := applicationArgs0; // regBegin
+  RefToInt[ApplicationArgs[CurrentTxn][0]] := 42;
+  ApplicationArgs[CurrentTxn][1] := applicationArgs1; // regEnd
+  RefToInt[ApplicationArgs[CurrentTxn][1]] := 42;
+  ApplicationArgs[CurrentTxn][2] := applicationArgs2; // voteBegin
+  RefToInt[ApplicationArgs[CurrentTxn][2]] := 42;
+  ApplicationArgs[CurrentTxn][3] := applicationArgs3; // voteEnd
+  RefToInt[ApplicationArgs[CurrentTxn][3]] := 42;
+
+  GroupSize := 1;
+  call contract();
+}
+
+procedure verifyDeleteApplication();
+implementation verifyDeleteApplication() {
+  var numAppArgs : Ref;
+  var onCompletion : Ref;
+  var applicationID : Ref;
+
+  call numAppArgs := FreshRefGenerator();
+  call applicationID := FreshRefGenerator();
+  call onCompletion := FreshRefGenerator();
+
+  IsInt[applicationID] := true;
+  ApplicationID[CurrentTxn] := applicationID;
+  assume RefToInt[ApplicationID[CurrentTxn]] != 0;
+
+  Sender[CurrentTxn] := Creator;
+
+  IsInt[numAppArgs] := true;
+  NumAppArgs[CurrentTxn] := numAppArgs;
+  RefToInt[NumAppArgs[CurrentTxn]] := 0;
+
+  IsInt[onCompletion] := true;
+  OnCompletion[CurrentTxn] := onCompletion;
+  RefToInt[OnCompletion[CurrentTxn]] := DeleteApplication;
+
+  GroupSize := 1;
+  call contract();
+}
+
+procedure verifyUpdateApplication();
+implementation verifyUpdateApplication() {
+  var numAppArgs : Ref;
+  var onCompletion : Ref;
+  var applicationID : Ref;
+
+  call numAppArgs := FreshRefGenerator();
+  call applicationID := FreshRefGenerator();
+  call onCompletion := FreshRefGenerator();
+
+  IsInt[applicationID] := true;
+  ApplicationID[CurrentTxn] := applicationID;
+  assume RefToInt[ApplicationID[CurrentTxn]] != 0;
+
+  Sender[CurrentTxn] := Creator;
+
+  IsInt[numAppArgs] := true;
+  NumAppArgs[CurrentTxn] := numAppArgs;
+  RefToInt[NumAppArgs[CurrentTxn]] := 0;
+
+  IsInt[onCompletion] := true;
+  OnCompletion[CurrentTxn] := onCompletion;
+  RefToInt[OnCompletion[CurrentTxn]] := UpdateApplication;
+
+  GroupSize := 1;
+  call contract();
+}
+
+procedure verifyCloseOut();
+implementation verifyCloseOut() {
+  var numAppArgs : Ref;
+  var onCompletion : Ref;
+  var applicationID : Ref;
+
+  call numAppArgs := FreshRefGenerator();
+  call applicationID := FreshRefGenerator();
+  call onCompletion := FreshRefGenerator();
+
+  IsInt[applicationID] := true;
+  ApplicationID[CurrentTxn] := applicationID;
+  assume RefToInt[ApplicationID[CurrentTxn]] != 0;
+
+  Sender[CurrentTxn] := Creator;
+
+  IsInt[numAppArgs] := true;
+  NumAppArgs[CurrentTxn] := numAppArgs;
+  RefToInt[NumAppArgs[CurrentTxn]] := 0;
+
+  IsInt[onCompletion] := true;
+  OnCompletion[CurrentTxn] := onCompletion;
+  RefToInt[OnCompletion[CurrentTxn]] := CloseOut;
+
+  GroupSize := 1;
+  call contract();
+}
+
+procedure verifyRegister();
+implementation verifyRegister() {
+  var numAppArgs : Ref;
+  var onCompletion : Ref;
+  var applicationID : Ref;
+
+  call numAppArgs := FreshRefGenerator();
+  call applicationID := FreshRefGenerator();
+  call onCompletion := FreshRefGenerator();
+
+  IsInt[applicationID] := true;
+  ApplicationID[CurrentTxn] := applicationID;
+  assume RefToInt[ApplicationID[CurrentTxn]] != 0;
+
+  Sender[CurrentTxn] := NotCreator;
+
+  IsInt[numAppArgs] := true;
+  NumAppArgs[CurrentTxn] := numAppArgs;
+  RefToInt[NumAppArgs[CurrentTxn]] := 1;
+
+  IsInt[onCompletion] := true;
+  OnCompletion[CurrentTxn] := onCompletion;
+  RefToInt[OnCompletion[CurrentTxn]] := OptIn;
+
+  ApplicationArgs[CurrentTxn][0] := register;
+
+  assume RefToInt[Globals[regBegin]] >= Round;
+  assume RefToInt[Globals[regEnd]] <= Round;
+
+  GroupSize := 1;
+  call contract();
+}
+
+procedure verifyVote();
+implementation verifyVote() {
+  var numAppArgs : Ref;
+  var onCompletion : Ref;
+  var applicationID : Ref;
+  var hardcodedToken : Ref;
+  var assetAmount : Ref;
+
+  call numAppArgs := FreshRefGenerator();
+  call applicationID := FreshRefGenerator();
+  call onCompletion := FreshRefGenerator();
+  call hardcodedToken := FreshRefGenerator();
+  call assetAmount := FreshRefGenerator();
+
+  IsInt[applicationID] := true;
+  ApplicationID[CurrentTxn] := applicationID;
+  assume RefToInt[ApplicationID[CurrentTxn]] != 0;
+
+  Sender[CurrentTxn] := NotCreator;
+
+  IsInt[numAppArgs] := true;
+  NumAppArgs[CurrentTxn] := numAppArgs;
+  RefToInt[NumAppArgs[CurrentTxn]] := 2;
+
+  IsInt[onCompletion] := true;
+  OnCompletion[CurrentTxn] := onCompletion;
+  RefToInt[OnCompletion[CurrentTxn]] := OptIn;
+
+  ApplicationArgs[CurrentTxn][0] := vote;
+  ApplicationArgs[CurrentTxn][1] := candidatea;
+
+  assume RefToInt[Globals[voteBegin]] >= Round;
+  assume RefToInt[Globals[voteEnd]] <= Round;
+  assume OptedInApp[NotCreator][RefToInt[applicationID]] >  0;
+  assume AssetBalance[NotCreator][RefToInt[hardcodedToken]] >= 1;
+  assume Accounts[CurrentTxn][0] == Sender[CurrentTxn];
+  IsInt[hardcodedToken] := true;
+  assume RefToInt[hardcodedToken] == 2;
+
+  GroupSize := 2;
+
+  TypeEnum[GroupTransaction[1]] := AssetTransfer;
+  AssetReceiver[GroupTransaction[1]] := Creator;
+
+  XferAsset[GroupTransaction[1]] := hardcodedToken;
+
+  IsInt[assetAmount] := true;
+  RefToInt[assetAmount] := 1;
+  AssetAmount[GroupTransaction[1]] := assetAmount;
+
+  call contract();
+}
